Finished implementing and cleaning up the code and getting it ready for submission

HeapInsert.dfy
@@ -1,308 +1,525 @@
+
 include "CCPR191-HeapSort-complete-30Dec18.dfy"
 
-method HeapInsert(a: array<int>, heapsize: nat, x: int)
+ method HeapInsert(a: array<int>, heapsize: nat, x: int)
 	requires heapsize < a.Length
 	requires hp(a[..], heapsize)
 	ensures hp(a[..], heapsize+1)
 	ensures multiset(a[..heapsize+1]) == multiset(old(a[..heapsize])+[x])
 	modifies a
-	{
+{	
 	assert heapsize < a.Length;
 	assert hp(a[..], heapsize);
 	assert ph(a[..], IndexSet(0, heapsize));
 
-	//alternation
-	if Guard1(heapsize)
-	{
-		HeapInsert1(a,heapsize,x);
+	a[heapsize] := x;
+	
+	Heapify(a,heapsize,x);
+
+	assert  hp(a[..], heapsize+1);
+	assert multiset(a[..heapsize+1]) == multiset(old(a[..heapsize])+[x]);
+}
+
+
+method Heapify(a: array<int>,heapsize: nat, x: int)
+	requires heapsize < a.Length
+	requires a[heapsize]==x
+	requires hp(a[..], heapsize)
+	requires ph(a[..], IndexSet(0, heapsize))
+	requires multiset(a[..heapsize+1]) == multiset(a[..heapsize]+[x])
+	ensures hp(a[..], heapsize+1)
+	ensures multiset(a[..heapsize+1]) == multiset(old(a[..heapsize])+[x])
+	modifies a
+{
+
+	assert ph(a[..], IndexSet(heapsize+1, heapsize+1));
+	assert ph(a[..], IndexSet(0, heapsize));
+	assert ph(a[..], IndexSet(heapsize, heapsize+1));
+	assert Inv(a,heapsize,x,heapsize,a[..heapsize],a[..heapsize]+[x]);
 		
+	
+	var  old_seq, old_seq2 := a[..heapsize], a[..heapsize+1];// introduce local variable
+	var j:nat := heapsize;// introduce local variable
+
+	assert ph(a[..], IndexSet(j+1, heapsize+1));
+	assert ph(a[..], IndexSet(0, j));
+	assert ph(a[..], IndexSet(j, heapsize+1));
+	assert Inv(a,heapsize,x,j,old_seq,old_seq2);
+
+	j := Loop(j,old_seq,old_seq2,a,heapsize,x);
+
+	assert  hp(a[..], heapsize+1);
+	assert multiset(a[..heapsize+1]) == multiset(old_seq+[x]);
+}
+
+
+
+
+method Loop(j0:nat,old_seq:seq<int>,old_seq2:seq<int>,a: array<int>,heapsize: nat, x: int) returns(j:nat)
+	requires j0 == heapsize < a.Length
+	requires Inv(a,heapsize,x,j0,old_seq,old_seq2)
+	ensures  Inv(a,heapsize,x,j,old_seq,old_seq2) && !(j!=0 && a[parent(j)] < a[j])
+	ensures  hp(a[..], heapsize+1);
+	ensures multiset(a[..heapsize+1]) == multiset(old_seq+[x]);
+	modifies a
+{//contract frame
+	j := j0;
+
+	assert j==heapsize;
+	assert Inv(a,heapsize,x,j,old_seq,old_seq2);
+	assert j==j0;
+	// iteration
+	while (j!=0 && a[parent(j)] < a[j])
+		invariant Inv(a,heapsize,x,j,old_seq,old_seq2) 
+		decreases j
+	{
+		j := Loop_Body(j,old_seq,old_seq2,a,heapsize,x);
+	}
+
+	assert Inv(a,heapsize,x,j,old_seq,old_seq2);
+	assert j ==0 || a[parent(j)] >= a[j]; // NOT of while guard
+			
+	Lemma_end_loop(a,heapsize,x,j,old_seq,old_seq2);
+	
+	assert  hp(a[..], heapsize+1);
+	assert multiset(a[..heapsize+1]) == multiset(old_seq+[x]);
+}
+
+method Loop_Body(j0:nat,old_seq:seq<int>,old_seq2:seq<int>,a: array<int>,heapsize: nat, x: int) returns(j:nat)
+	requires Inv(a,heapsize,x,j0,old_seq,old_seq2)
+	requires j0!=0 && a[(j0-1)/2] < a[j0]
+	ensures Inv(a,heapsize,x,j,old_seq,old_seq2)
+	ensures j0 > j >= 0
+	modifies a
+{//contract frame 
+	assert Inv(a,heapsize,x,j0,old_seq,old_seq2);
+	j:=j0; 
+
+	assert Inv(a,heapsize,x,j,old_seq,old_seq2) ==> (0 < j <= heapsize < a.Length);
+	assert Inv(a,heapsize,x,j,old_seq,old_seq2) ==> ph(a[..], IndexSet(0, j)) && ph(a[..], IndexSet(j, heapsize+1));
+
+	Swap(a, parent(j), j,heapsize,x,old_seq,old_seq2);
+
+	assert Inv(a,heapsize,x,parent(j),old_seq,old_seq2);
+
+	j := parent(j);
+		
+	assert Inv(a,heapsize,x,j,old_seq,old_seq2);
+}
+
+
+lemma Lemma_end_loop(a: array<int>,heapsize: nat, x: int , j:nat , old_seq:seq<int>,old_seq2:seq<int>)
+	requires Inv(a,heapsize,x,j,old_seq,old_seq2)
+	requires j==0 || a[parent(j)] >= a[j]
+	requires ph(a[..], IndexSet(0, j)) && ph(a[..], IndexSet(j, heapsize+1)) && ph(a[..], IndexSet(0, heapsize+1)-{j}) 
+	ensures  hp(a[..], heapsize+1)
+	ensures multiset(a[..heapsize+1]) == multiset(old_seq+[x]);
+{	
+	//alternation
+	if(j == 0)
+	{
+		assert j == 0;
+		//==>
+		assert ph(a[..], IndexSet(0, heapsize+1)); // by pre condition
+		//==>
+		assert hp(a[..], heapsize+1);
+		assert multiset(a[..heapsize+1]) == multiset(old_seq+[x]) by { assert Inv(a,heapsize,x,j,old_seq,old_seq2); /* pre cond. */}
 	}
 	else
 	{
-		HeapInsert2(a,heapsize,x);
-		
-	}	
-	assert ph(a[..], IndexSet(0,heapsize+1));	
-	assert  hp(a[..], heapsize+1);
-	assert multiset(a[..heapsize+1]) == multiset(old(a[..heapsize])+[x]);
+		assert ph(a[..], IndexSet(0, j)); // pre condition
+		//==>
+		assert hp(a[..], j);
+
+		assert a[parent(j)] >= a[j]; // pre condition (else part)
+		//==>		
+		assert hp(a[..], j+1) by { Lemma_end_loop1(a, j); }
+		assert multiset(a[..heapsize+1]) == multiset(old_seq+[x]) by { assert Inv(a,heapsize,x,j,old_seq,old_seq2); /* pre cond. */}
 	}
 
-	predicate method Guard1(heapsize:nat)
-{
-	heapsize == 0
+	assert hp(a[..], heapsize+1);
+	assert multiset(a[..heapsize+1]) == multiset(old_seq+[x]);
 }
 
-	method HeapInsert1(a: array<int>, heapsize: nat, x: int)
-	requires Guard1(heapsize);
-	requires heapsize < a.Length
-	requires hp(a[..], heapsize)
-	requires ph(a[..], IndexSet(0, heapsize))
-	ensures a[heapsize]==x;
-	ensures hp(a[..], heapsize+1)
-	ensures multiset(a[..heapsize+1]) == multiset(old(a[..heapsize])+[x])
-	ensures ph(a[..], IndexSet(0, heapsize+1))
-	modifies a
-	{
-		Lemmax(a, heapsize, x);//assignemnt
-		a[heapsize]:=x;
-	}
+function method parent(j: nat): nat
+	requires 0 < j 
+{
+	(j-1)/2
+}
 
+function IndexAncestorsSet(start: nat, end: nat, j: nat): set<nat>
+{
+	set i: nat | i < end && InRange(start, i, end) && AncestorIndex(i, j)
+}
 
-	lemma Lemmax (a: array<int>, heapsize: nat, x: int)
-	requires Guard1(heapsize);
-	requires heapsize < a.Length
-	requires hp(a[..], heapsize)
-	requires ph(a[..], IndexSet(0, heapsize))
-	ensures hp(a[..], heapsize+1)
-	ensures multiset(a[..heapsize+1][heapsize := x]) == multiset(old(a[..heapsize])+[x])
-	ensures ph(a[..], IndexSet(0, heapsize+1))
-	{
-	}
-
-	lemma Lemmax2 (a: array<int>, heapsize: nat, x: int)
-	requires !Guard1(heapsize);
-	requires heapsize < a.Length
-	requires hp(a[..], heapsize)
-	requires ph(a[..], IndexSet(0, heapsize))
-
-	ensures 0 < heapsize < a.Length
-	ensures multiset(a[..heapsize+1][heapsize := x]) == multiset(a[..heapsize]+[x])
-	ensures hp(a[..], heapsize)
-	ensures ph(a[..], IndexSet(0, heapsize))
-	
-	{
-	}
-
-	
-	method HeapInsert2(a: array<int>, heapsize: nat, x: int)
-	requires !Guard1(heapsize);
-	requires heapsize < a.Length
-	requires hp(a[..], heapsize)
-	requires ph(a[..], IndexSet(0, heapsize))
-	ensures hp(a[..], heapsize+1)
-	ensures multiset(a[..heapsize+1]) == multiset(old(a[..heapsize])+[x])
-	ensures ph(a[..], IndexSet(0, heapsize+1))
-	modifies a
-	{
-		Lemmax2(a, heapsize, x);//assignemnt
-		a[heapsize]:=x;
-		Heapify(a,heapsize,x);
-	}
-
-
-	method Heapify(a: array<int>,heapsize: nat, x: int)
+lemma Lemma_end_loop1(a: array<int>, heapsize: nat)
 	requires 0 < heapsize < a.Length
-	requires multiset(a[..heapsize+1]) == multiset(a[..heapsize]+[x])
 	requires hp(a[..], heapsize)
-	requires a[heapsize]==x
-	requires ph(a[..], IndexSet(0, heapsize))
-
+	requires a[parent(heapsize)] >= a[heapsize];
 	ensures hp(a[..], heapsize+1)
-	ensures ph(a[..], IndexSet(0, heapsize+1))
-	ensures multiset(a[..heapsize+1]) == multiset(old(a[..heapsize])+[x])
-	modifies a;
-	{
-
-
-
-	var j,old_j,old_seq,old_seq2,i:=Init_Heapify(a,heapsize, x);
-	i,old_j,j:=Loop(j,old_j,old_seq,old_seq2,i,a,heapsize,x);
-	
-
-	assert Inv(a,heapsize,x,j,old_seq,old_seq2);
-
-
-	assert !(j > 0 && a[(j-1)/2] < a[j]);
-	assert j==0 ||  a[(j-1)/2] >= a[j];
-	
-
-	assert Inv(a,heapsize,x,j,old_seq,old_seq2);
-	
-	assert forall j:int ::
-	0<=j<heapsize+1<=a.Length && (j == 0 || (j>0 && a[(j-1)/2] >= a[j])) && Inv(a,heapsize,x,j,old_seq,old_seq2) ==> 
-	hp(a[..], j) && ph(a[..], IndexSet(0, j)) && ph(a[..], IndexSet(j, heapsize+1));
-
-
-	assert ph(a[..], IndexSet(0, j)) && ph(a[..], IndexSet(j, heapsize+1));
-	
-	assert forall j:int ::
-	0<=j<heapsize+1<=a.Length && (j == 0 || (j>0 && a[(j-1)/2] >= a[j])) && ph(a[..], IndexSet(0, j)) 
-	&& ph(a[..], IndexSet(j, heapsize+1)) && Inv(a,heapsize,x,j,old_seq,old_seq2) 
-	==> ph(a[..], IndexSet(0, heapsize+1)) && multiset(a[..heapsize+1]) == multiset(old_seq2+[x]);
-	
-	assert ph(a[..], IndexSet(0, heapsize+1));
-	assert  hp(a[..], heapsize+1);
-	assert multiset(a[..heapsize+1]) == multiset(old_seq2+[x]);
-	
-	}
-
-
-
-method Loop(j0:nat,old_j0:nat,old_seq:seq<int>,old_seq2:seq<int>,i0:nat,a: array<int>,heapsize: nat, x: int) returns(i:nat,old_j:nat,j:nat)
-requires j0==heapsize;
-requires old_j0 == heapsize+1;
-requires i0 == (j0-1)/2;
-requires  0< j0 <= heapsize < a.Length;
-requires Inv(a,heapsize,x,j0,old_seq,old_seq2);
-ensures j<=j0 
-ensures Inv(a,heapsize,x,j,old_seq,old_seq2) &&  (j==0 ||  a[(j-1)/2] >= a[j])
-modifies a;
 {
-
-j:=j0;
-old_j:=old_j0;
-i:=i0;
-assert j==heapsize;
-assert old_j == heapsize+1;
-assert i == (j-1)/2;
-assert  0< j <= heapsize < a.Length;
-assert Inv(a,heapsize,x,j,old_seq,old_seq2);
-
- while (j!=0 && a[(j-1)/2] < a[j])
-		invariant Inv(a,heapsize,x,j,old_seq,old_seq2);
-		decreases j
-   
-    {
-		
-		assert Inv(a,heapsize,x,j,old_seq,old_seq2);
-		
-		assert forall j:int ::
-		0<=j<heapsize+1<=a.Length && (j > 0 && a[(j-1)/2] < a[j]) && Inv(a,heapsize,x,j,old_seq,old_seq2) ==> 
-		hp(a[..], j) && ph(a[..], IndexSet(0, j)) && ph(a[..], IndexSet(j, heapsize+1));
-
-		assert 0 < j <= heapsize && 0 < heapsize < a.Length && hp(a[..], j) && ph(a[..], IndexSet(0, j)) && ph(a[..], IndexSet(j, heapsize+1));
-				 
-		var old1:=a[(j-1)/2]; 
-		var old2:=a[j];
-		var old_set:= multiset(a[..heapsize+1]);
-		
-		  i := (j-1)/2;
-		
-		assert ph(a[..], IndexSet(0, j));
-		assert ph(a[..], IndexSet(j+1, heapsize+1));
-		assert ph(a[..], IndexSet(0, i));
-
-
-		assert ph(a[..], IndexSet(0, j));
-		assert j <= heapsize;
-		assert j == (old_j-1)/2 || (j == heapsize && old_j == heapsize+1);
-		
-
-		assert j<=heapsize;
-
-	
-		
-		assert ph(a[..], IndexSet(0, j));
-		assert ph(a[..], IndexSet(j, heapsize+1));
-		assert ph(a[..], IndexSet(j, old_j));
-		
-		Swap(a, i, j,heapsize);
-	
-		assert ph(a[..], IndexSet(0, i));
-		assert ph(a[..], IndexSet(i+1, heapsize+1));
-		assert ph(a[..], IndexSet(i, j));
-
-		assert  a[i]==old2;
-		assert a[j]==old1;
-		assert old_set == multiset(a[..heapsize+1]);
-	
-
-		  old_j := j;
-	  	   j := i;
-
-		
-		assert j == (old_j-1)/2;
-		
-		assert Inv(a,heapsize,x,j,old_seq,old_seq2);
-		assert ph(a[..], IndexSet(0, j)) && ph(a[..], IndexSet(j, heapsize+1));
-
-	}
-	assert Inv(a,heapsize,x,j,old_seq,old_seq2) &&  (j==0 ||  a[(j-1)/2] >= a[j]);
-	
-}
-
-
-method  Init_Heapify(a: array<int>,heapsize: nat, x: int) returns (j:nat,old_j:nat,old_seq:seq<int>,old_seq2:seq<int>,i:nat)
-requires 0 < heapsize < a.Length
-	requires multiset(a[..heapsize+1]) == multiset(a[..heapsize]+[x])
-	requires hp(a[..], heapsize)
-	requires a[heapsize]==x
-	requires ph(a[..], IndexSet(0, heapsize))
-	ensures j==heapsize;
-	ensures old_j == heapsize+1;
-	ensures i == (j-1)/2;
-	ensures 0<j<=heapsize<a.Length;
-
-	ensures Inv(a,heapsize,x,j,old_seq,old_seq2);
-{
-	assert  0 < heapsize < a.Length;
-	assert multiset(a[..heapsize+1]) == multiset(a[..heapsize]+[x]);
 	assert hp(a[..], heapsize);
-	assert a[heapsize]==x;
-	assert ph(a[..], IndexSet(0, heapsize));
-	
-	assert ph(a[..], IndexSet(heapsize+1, heapsize+1));
+	//<==>
+	assert forall i,j :: 0 <= i < heapsize && 0 <= j < heapsize && AncestorIndex(i, j) ==> a[..][i] >= a[..][j];
+	assert a[parent(heapsize)] >= a[heapsize];
+	//==>
+	assert hp(a[..], parent(heapsize));
+	//==>
+	assert forall i :: 0 <= i < heapsize && AncestorIndex(i, parent(heapsize)) ==> a[..][i] >= a[..][parent(heapsize)];
+	assert a[parent(heapsize)] >= a[heapsize];
+	//==>
+	ghost var s1 := IndexAncestorsSet(0, heapsize+1, parent(heapsize));
+	ghost var s2 := IndexAncestorsSet(0, heapsize+1, heapsize);
 
-     j:=heapsize;
+	assert forall i:: i in s1 ==> a[i] >= a[parent(heapsize)];
 
-	assert ph(a[..], IndexSet(j+1, heapsize+1));
-  
-	  old_j := heapsize+1;
-	assert old_j >= j;
+	L2(heapsize);
 
-	 old_seq:= a[..heapsize];
-	 old_seq2:= a[..heapsize+1];
+	assert s2 == s1 + {heapsize};
+	//==>
+	assert forall i:: i in s2 ==> a[i] >= a[heapsize];
 
-	assert ph(a[..], IndexSet(0, j));
-	assert ph(a[..], IndexSet(j, heapsize+1));
-	assert ph(a[..], IndexSet(j, old_j));
-
-	 i := (j-1)/2;
-	assert j == heapsize;
-	assert j == heapsize && old_j == heapsize+1;
+	assert forall i :: 0 <= i < heapsize && AncestorIndex(i, heapsize) ==> a[..][i] >= a[..][heapsize];
+	//==>
+	assert forall i,j :: 0 <= i < heapsize && 0 <= j <= heapsize && AncestorIndex(i, j) ==> a[..][i] >= a[..][j];
+	//==>
+	assert forall i,j :: 0 <= i <= heapsize && 0 <= j <= heapsize && AncestorIndex(i, j) ==> a[..][i] >= a[..][j];
+	//<==>
+	assert hp(a[..], heapsize+1);
 }
 
-
-method Swap(a: array<int>,  i: int, j: nat,heapsize:nat)
-  requires 0 <= i < j <= heapsize < a.Length
-  requires  a[i] < a[j]
-  requires ph(a[..], IndexSet(0, i))
-  requires ph(a[..], IndexSet(0, j))
-  requires ph(a[..], IndexSet(j+1, heapsize+1))
-
-  ensures a[i] == old(a[j]);
-  ensures a[j] == old(a[i]);
-  ensures forall m :: heapsize < m < a.Length && m != i && m != j ==> a[m] == old(a[m]);
-  ensures a[..i] == old(a[..i])
-  ensures ph(a[..], IndexSet(0, i))
-  ensures a[i+1..j] == old(a[i+1..j])
-  ensures ph(a[..], IndexSet(i, j))
-  ensures a[j+1..] == old(a[j+1..])
-  ensures ph(a[..], IndexSet(j+1, heapsize+1))
-  ensures multiset(a[..heapsize+1]) == old(multiset(a[..heapsize+1]));
-  modifies a;
+lemma L2(j: nat)
+	requires 0 < j
+	ensures IndexAncestorsSet(0, j+1, j) == IndexAncestorsSet(0, j+1, parent(j)) + {j}
 {
-  a[i], a[j] := a[j], a[i];
+	calc
+	{
+		IndexAncestorsSet(0, j+1, j);
+	== 
+		IndexAncestorsSet(0, parent(j)+1, j) + IndexAncestorsSet(parent(j)+1, j+1, j);
+	== { L3(j); }
+		IndexAncestorsSet(0, parent(j)+1, parent(j)) + IndexAncestorsSet(parent(j)+1, j+1, j);
+	==
+		IndexAncestorsSet(0, j+1, parent(j)) + IndexAncestorsSet(parent(j)+1, j+1, j);
+	== 
+		IndexAncestorsSet(0, j+1, parent(j)) + {j};
+	}
 }
 
+lemma L3(j: nat)
+	requires 0 < j
+	ensures IndexAncestorsSet(0, parent(j)+1, j) == IndexAncestorsSet(0, parent(j)+1, parent(j))
+{
+	var s1 := IndexAncestorsSet(0, parent(j)+1, j);
+	var s2 := IndexAncestorsSet(0, parent(j)+1, parent(j));
+	
+	assert s1 <= s2 by { L4(j); }
+	assert s1 >= s2 by { L5(j); }
+	//==>
+	assert s1 ==s2;
+	//==>
+	assert IndexAncestorsSet(0, parent(j)+1, j) == IndexAncestorsSet(0, parent(j)+1, parent(j));
+}
 
+lemma L4(j: nat)
+	requires 0 < j
+	ensures IndexAncestorsSet(0, parent(j)+1, j) <= IndexAncestorsSet(0, parent(j)+1, parent(j))
+{
+	forall i | 0 <= i < j && AncestorIndex(i, j) ensures AncestorIndex(i, parent(j)) {
+		L4step(i, j);
+	}
+	//==>
+	assert forall i :: 0 <= i < j && AncestorIndex(i, j) ==> AncestorIndex(i, parent(j));
+	//==>
+	assert IndexAncestorsSet(0, parent(j)+1, j) <= IndexAncestorsSet(0, parent(j)+1, parent(j));
+}
+
+lemma L4step(i: nat, j: nat)
+	requires 0 <= i < j
+	requires AncestorIndex(i, j)
+	ensures AncestorIndex(i, parent(j))
+	decreases j-i
+{
+	assert AncestorIndex(i, j);
+	//<==> def.
+	assert i == j || (j > 2*i && ((AncestorIndex(2*i+1, j) || AncestorIndex(2*i+2, j))));
+	//==>
+	if(i == j)//alternation
+	{
+		assert AncestorIndex(j, j);
+		//==>
+		assert AncestorIndex(j, parent(j)) by { assert parent(j) < j; }
+		//==>
+		assert AncestorIndex(i, parent(j));
+	}
+	else
+	{
+		assert j > 2*i && ((AncestorIndex(2*i+1, j) || AncestorIndex(2*i+2, j)));
+		
+		if AncestorIndex(2*i+1, j)//alternation
+		{
+			assert parent(2*i+1) == i;
+			//==> 2*i+1 is a child of i
+			//==> i is at least grand parent of j
+			assert AncestorIndex(i, parent(j));
+		}
+		else
+		{
+			assert AncestorIndex(2*i+2, j);
+			assert parent(2*i+2) == i;
+			//==> 2*i+2 is a child of i
+			//==> i is at least grand parent of j
+			assert AncestorIndex(i, parent(j));
+		}
+		
+		assert AncestorIndex(i, parent(j));
+	}
+
+	assert AncestorIndex(i, parent(j));
+}
+
+lemma L5(j: nat)
+	requires 0 < j
+	ensures IndexAncestorsSet(0, parent(j)+1, j) >= IndexAncestorsSet(0, parent(j)+1, parent(j))
+{
+	forall i | 0 <= i < j && AncestorIndex(i, parent(j)) ensures AncestorIndex(i, j) {
+		L5step(i, j);
+	}
+	//==>
+	assert forall i:: 0 <= i < j && AncestorIndex(i, parent(j)) ==> AncestorIndex(i, j);
+	//==>
+	assert IndexAncestorsSet(0, parent(j)+1, j) >= IndexAncestorsSet(0, parent(j)+1, parent(j));
+}
+
+lemma L5step(i: nat, j: nat)
+	requires 0 <= i < j
+	requires AncestorIndex(i, parent(j))
+	ensures AncestorIndex(i, j)
+	decreases j-i
+{
+	assert AncestorIndex(i, parent(j));
+	//<==> def.
+	assert i == parent(j) || (parent(j) > 2*i && ((AncestorIndex(2*i+1, parent(j)) || AncestorIndex(2*i+2, parent(j)))));
+	//==>
+	if(i == parent(j))//alternation
+	{
+		assert AncestorIndex(parent(j), j);
+		//==>
+		assert AncestorIndex(i, j);
+	}
+	else
+	{
+		assert parent(j) > 2*i && ((AncestorIndex(2*i+1, parent(j)) || AncestorIndex(2*i+2, parent(j))));
+		
+		if AncestorIndex(2*i+1, parent(j))//alternation
+		{
+			assert parent(2*i+1) == i;
+			//==> 2*i+1 is a child of i
+			assert AncestorIndex(i, j);
+		}
+		else
+		{
+			assert AncestorIndex(2*i+2, parent(j));
+			assert parent(2*i+2) == i;
+			//==> 2*i+2 is a child of i
+			assert AncestorIndex(i, j);
+		}
+		
+		assert AncestorIndex(i, j);
+	}
+
+	assert AncestorIndex(i, j);
+}
+
+method Swap(a: array<int>, i: int, j: nat,heapsize:nat, x:int,old_seq:seq<int>,old_seq2:seq<int>)
+	requires 0 <= i < j <= heapsize < a.Length && heapsize == |old_seq| && |old_seq2|==heapsize+1
+	requires i == parent(j)
+	requires  a[i] < a[j] == x
+	requires Inv(a,heapsize,x,j,old_seq,old_seq2)
+
+	ensures x == a[i] > a[j]
+	ensures Inv(a,heapsize,x,i,old_seq,old_seq2)
+	modifies a
+{
+	SwapProof(a,i,j,heapsize,x,old_seq,old_seq2);
+
+	a[i], a[j] := a[j], a[i];
+
+	assert  SemiHeapPred(a,heapsize,i);
+	InvProof(a,i,j,heapsize,x,old_seq,old_seq2);		
+	//==>
+	assert Inv(a,heapsize,x,i,old_seq,old_seq2);
+}
+
+lemma SwapProof(a: array<int>, i: int, j: nat,heapsize:nat, x:int,old_seq:seq<int>,old_seq2:seq<int>)
+	requires 0 <= i < j <= heapsize < a.Length && i == parent(j)
+	requires IntegPred(a,heapsize,j,x,old_seq,old_seq2)
+	requires a[i] < a[j]==x
+	requires SemiHeapPred(a,heapsize,j)
+	ensures var q := a[..][i := a[j]][j := a[i]];  
+		&& ph(q[..], IndexSet(0, i))
+		&& ph(q[..], IndexSet(i, heapsize+1))
+		&& ph(q[..], IndexSet(0, heapsize+1) - {i})
+		&& q[..i]==a[..i] && q[i]==x
+		&& multiset(q[..i+1]) == multiset(a[..i]+[x]) 
+		&& multiset(q[..heapsize+1]) == multiset(old_seq2) == multiset(old_seq+[x]) 
+		&& multiset(q[..heapsize+1]) == multiset(q[..heapsize+1]) 
+
+{
+	var q := a[..][i := a[j]][j := a[i]];
+
+	assert ph(q[..], IndexSet(0, i)) by { LemmaMaxLowerHeap(a,i,j,heapsize,x,old_seq,old_seq2);}
+	assert ph(q[..], IndexSet(i, heapsize+1)) by { LemmaMaxUpperHeap(a,i,j,heapsize,x,old_seq,old_seq2); }
+	assert multiset(a[..heapsize+1]) == multiset(q[..heapsize+1]) by { LemmaSwapMaintainsMultiset(a[..],q[..],i,j); }
+	assert ph(q[..], IndexSet(0, heapsize+1) - {i}) by{ LemmaPhWithoutI(a,i,j,heapsize,x,old_seq,old_seq2); }
+}
+
+lemma LemmaPhWithoutI(a: array<int>, i: int, j: nat,heapsize:nat, x:int,old_seq:seq<int>,old_seq2:seq<int>)
+	requires 0 <= i < j <= heapsize < a.Length && i == parent(j)
+	requires IntegPred(a,heapsize,j,x,old_seq,old_seq2)
+	requires a[i] < a[j] == x
+	requires SemiHeapPred(a,heapsize,j)
+	ensures var q := a[..][i := a[j]][j := a[i]]; ph(q[..], IndexSet(0, heapsize+1) - {i}) 
+{	
+	var q := a[..][parent(j) := a[j]][j := a[parent(j)]];			
+			
+	forall m | m in  IndexSet(0, heapsize+1) && AncestorIndex(m,j) ensures q[m]>=q[j] {
+		// Pre conds.
+		assert 0 < j <= heapsize < a.Length;
+		assert a[parent(j)] < a[j];
+		assert SemiHeapPred(a,heapsize,j);
+
+		// above assignment
+		assert q == a[..][parent(j) := a[j]][j := a[parent(j)]];
+
+		// forall condition
+		assert m in  IndexSet(0, heapsize+1) && AncestorIndex(m,j);
+
+		//==>
+		LemmaPhWithoutIstep(a, j, heapsize, m, q);
+	}
+	//==>
+	assert forall m :: m in  IndexSet(0, heapsize+1) && AncestorIndex(m,j) ==> q[m]>=q[j];
+	//==>
+	assert forall l,k:: l in  IndexSet(0, heapsize+1) && k in  IndexSet(0, heapsize+1) && AncestorIndex(l,k) && l!=i && k!=i ==>  q[l] >= q[k];
+	assert (forall l,k:: l in  IndexSet(0, heapsize+1) && k in  IndexSet(0, heapsize+1) && AncestorIndex(l,k) && l!=i && k!=i ==>  q[l] >= q[k])==> ph(q[..], IndexSet(0, heapsize+1) - {i});
+	//==>
+	assert var q := a[..][i := a[j]][j := a[i]]; ph(q[..], IndexSet(0, heapsize+1) - {i});
+}
+
+lemma LemmaPhWithoutIstep(a: array<int>, j: nat,heapsize:nat, m:nat, q:seq<int>)
+	requires 0 < j <= heapsize < a.Length
+	requires a[parent(j)] < a[j]
+	requires m in  IndexSet(0, heapsize+1) && AncestorIndex(m,j)
+	requires q == a[..][parent(j) := a[j]][j := a[parent(j)]]
+	requires SemiHeapPred(a,heapsize,j);
+	ensures q[m]>=q[j]
+{
+	assert AncestorIndex(m,j);
+	//==>
+	if(m == j)//alternation
+	{
+		// Trivial
+		assert q[m]>=q[j];
+	}
+	else // m is at least the parent of j
+	{
+		assert ph(a[..], IndexSet(0, j)) by { assert SemiHeapPred(a,heapsize,j); /* pre cond. */}
+		assert a[parent(j)] < a[j]; // pre cond.
+		//==>
+		assert q[parent(j)] >= q[j]; // swapped
+		
+		assert AncestorIndex(parent(j), j);
+		//==>
+
+		assert AncestorIndex(m, parent(j)) by { L4step(m, j); }
+		//==>
+		assert q[m]>=q[j];
+	}
+	assert q[m]>=q[j];
+}
+
+lemma LemmaMaxLowerHeap(a: array<int>, i: int, j: nat,heapsize:nat, x:int,old_seq:seq<int>,old_seq2:seq<int>)
+	requires 0 <= i < j <= heapsize < a.Length  
+	requires i == parent(j)
+	requires  a[i] < a[j]
+	requires ph(a[..], IndexSet(0, j))
+	ensures var q := a[..][i := a[j]][j := a[i]]; ph(q[..], IndexSet(0, i))
+{
+	var q := a[..][i := a[j]][j := a[i]]; 
+	assert ph(q[..], IndexSet(0, i));
+}
+
+lemma LemmaMaxUpperHeap(a: array<int>, i: int, j: nat,heapsize:nat, x:int,old_seq:seq<int>,old_seq2:seq<int>)
+	requires 0 <= i < j <= heapsize < a.Length  
+	requires i == parent(j)
+	requires a[i] < a[j]
+	requires ph(a[..], IndexSet(0, j))
+	requires ph(a[..], IndexSet(j, heapsize+1))
+	requires ph(a[..], IndexSet(0, heapsize+1) - {j})
+	ensures var q := a[..][i := a[j]][j := a[i]]; 
+		&& ph(q[..], IndexSet(i, heapsize+1)) 
+{ 
+	var q := a[..][i := a[j]][j := a[i]]; 
+	assert ph(q[..], IndexSet(i, heapsize+1));
+}
+
+lemma InvProof(a: array<int>, i: nat, j: nat,heapsize:nat, x:int,old_seq:seq<int>,old_seq2:seq<int>)
+	requires 0 <= i < j <= heapsize < a.Length &&  i == parent(j) 
+	requires|old_seq|==|a[..heapsize]| && |old_seq2|==heapsize+1
+	requires SemiHeapPred(a,heapsize,i)
+	requires x == a[i] > a[j]
+	requires  multiset(a[..heapsize+1]) == multiset(old_seq2)
+	requires a[i]==x
+		&& multiset(a[..i+1]) == multiset(a[..i]+[x]) 
+		&& multiset(a[..heapsize+1]) == multiset(old_seq2) == multiset(old_seq+[x]) 
+		&& multiset(a[..heapsize+1]) == multiset(a[..heapsize+1]) 
+	requires hp(old_seq2,heapsize)
+	ensures Inv(a,heapsize,x,i,old_seq,old_seq2)
+{
+	assert IntegPred(a,heapsize,i,x,old_seq,old_seq2) ;
+}
 
 predicate Inv(a: array<int>,heapsize: nat, x: int , j:nat , old_seq:seq<int>,old_seq2:seq<int>)
-reads a;
+	reads a
 {
-	
-	0 < j <= heapsize && 
-	0 < heapsize < a.Length &&
-	hp(a[..], j) && 
-	
-	ph(a[..], IndexSet(0, j))&&
-	ph(a[..], IndexSet(j, heapsize+1)) &&
-	
-	multiset(a[..j+1]) == multiset(a[..j]+[x]) &&
-	multiset(a[..heapsize+1]) == multiset(old_seq2) && 
-	j>0 ==> AncestorIndex((j-1)/2,j) &&
-	(forall k,h :: j < h <= k <= heapsize  && (k - 1) / 2 == j && j > 0 && AncestorIndex(h, k)  ==>  a[h] >= a[k])&&				
-	a[j]==x &&
-	multiset(a[..heapsize+1]) == multiset(old_seq+[x])
+	j <= heapsize < a.Length &&
+	a[j] == x &&
 
+	SemiHeapPred(a,heapsize,j) &&
+	IntegPred(a,heapsize,j,x,old_seq,old_seq2) &&
+	BigJPred(a, heapsize, j, x, old_seq) && 
+		
+	|old_seq|==|a[..heapsize]| &&
+	|old_seq2|==heapsize+1 && 
+	hp(old_seq2,heapsize)
+}
+
+predicate BigJPred(a:array<int>, heapsize:nat, j:nat, x:int, old_seq:seq<int>)
+	reads a	
+{
+	j>0 ==>	AncestorIndex(parent(j),j) &&
+
+	forall i, h ::
+		0 <= i < parent(j) == j < h <= heapsize && 
+		AncestorIndex(h, heapsize) && 
+		AncestorIndex(i, j-1) 
+	==> 
+		a[h] >= a[heapsize]  &&  a[i] >= a[j-1]
+}
+	
+predicate SemiHeapPred(a:array<int>, heapsize:nat, j:nat)
+	reads a
+{
+	j <= heapsize < a.Length && 
+	ph(a[..], IndexSet(0, j))&& ph(a[..], IndexSet(j, heapsize+1)) &&  
+	ph(a[..], IndexSet(0, heapsize+1)-{j})
+}
+	
+predicate IntegPred(a:array<int>, heapsize:nat, j:nat, x:int, old_seq:seq<int>, old_seq2:seq<int>)
+	reads a
+{
+	j <= heapsize < a.Length &&
+	multiset(a[..j+1]) == multiset(a[..j]+[x]) &&
+	multiset(a[..heapsize+1]) == multiset(old_seq2) == multiset(old_seq+[x]) 
 }
